type_system/type_lemmas.v
@@ -10,8 +10,6 @@ Add LoadPath "C:\Users\Ziga\Documents\Ziga_podatki\repositories\eeff-formalizati
 (* Add LoadPath "E:\Ziga_Podatki\faks\eeff-formalization\logic". *)
 Require Export type_aux_lemmas operational_semantics.
 
-Ltac inv H := inversion H; clear H; subst.
-
 (* ==================== Substitution Lemma ==================== *)
 
 Fixpoint v_subs_out_typesafe Γ v A v_s A_s {struct v}:
@@ -25,19 +23,19 @@ with c_subs_out_typesafe Γ c C v_s A_s {struct c}:
 with h_subs_out_typesafe Γ h Σ D v_s A_s {struct h}:
   has_htype (CtxU Γ A_s) h Σ D -> has_vtype Γ v_s A_s ->
   has_htype Γ (h_subs_out h v_s) Σ D.
+
 Proof.
 {
 intros orig sub. unfold v_subs_out.
-assert (CtxU Γ A_s = ctx_insert Γ A_s 0) by (destruct Γ; auto).
+assert (CtxU Γ A_s = ctx_insert Γ 0 A_s) by (destruct Γ; auto).
 eapply v_subs_typesafe; eauto. destruct Γ; omega.
 }{
 intros orig sub. unfold c_subs_out.
-assert (CtxU Γ A_s = ctx_insert Γ A_s 0) by (destruct Γ; auto).
+assert (CtxU Γ A_s = ctx_insert Γ 0 A_s) by (destruct Γ; auto).
 eapply c_subs_typesafe; eauto. destruct Γ; omega.
 }{
 intros orig sub. unfold h_subs_out.
-assert (Γ = ctx_remove (CtxU Γ A_s) 0) by auto.
-assert (CtxU Γ A_s = ctx_insert Γ A_s 0) by (destruct Γ; auto).
+assert (CtxU Γ A_s = ctx_insert Γ 0 A_s) by (destruct Γ; auto).
 eapply h_subs_typesafe; eauto. destruct Γ; omega.
 }
 Qed.
@@ -49,20 +47,20 @@ Theorem preservation Γ c c' C:
 Proof.
 intros orig step. revert C orig. 
 induction step; intros C orig.
-+ unfold c_subs2_out. apply shape_prodmatch in orig.
-  destruct orig as [A [B [pair]]]. apply shape_pair in pair. destruct pair.
+all: try unfold c_subs2_out.
++ apply shape_prodmatch in orig. destruct orig as [A [B [pair]]].
+  apply shape_pair in pair. destruct pair.
   eapply c_subs_out_typesafe. eapply c_subs_out_typesafe.
   all: eauto. inv H0. apply v_shift_typesafe; auto.
-+ unfold c_subs2_out. apply shape_summatch in orig.
++ apply shape_summatch in orig.
   destruct orig as [A [B [vty [inl _]]]].
   eapply c_subs_out_typesafe. exact inl. apply shape_inl in vty. auto.
-+ unfold c_subs2_out. apply shape_summatch in orig.
++ apply shape_summatch in orig.
   destruct orig as [A [B [vty [_ inr]]]].
   eapply c_subs_out_typesafe. exact inr. apply shape_inr in vty. auto.
 + apply shape_listmatch in orig.
   destruct orig as [A[_[ty1 _]]]. auto.
-+ unfold c_subs2_out. 
-  apply shape_listmatch in orig. destruct orig as [A[vty[_ ty2]]]. 
++ apply shape_listmatch in orig. destruct orig as [A[vty[_ ty2]]]. 
   apply shape_cons in vty. destruct vty as [vty vsty].  
   eapply c_subs_out_typesafe; eauto. eapply c_subs_out_typesafe; eauto.
   eapply v_shift_typesafe; eauto. inv vty. auto.
@@ -70,56 +68,56 @@ induction step; intros C orig.
   eapply c_subs_out_typesafe; eauto.
 + apply shape_letrec in orig. destruct orig as [A [C' [c1ty]]].
   eapply c_subs_out_typesafe; eauto. apply TypeV. inv c1ty.
-  inv H. inv H3. assumption. inv H. inv H0. assumption.  
+  inv H. inv H3. auto. inv H. inv H0. auto.  
   apply TypeFun. apply TypeC. 
-  - inv c1ty. inv H0. assumption.
-  - inv c1ty. assumption.
+  - inv c1ty. inv H0. auto.
+  - inv c1ty. auto.
   - eapply TypeLetRec. 2: exact c1ty.
     assert (CtxU (CtxU (CtxU Γ A) A) (TyFun A C') 
-      = ctx_insert (CtxU (CtxU Γ A) (TyFun A C')) A 2)
+      = ctx_insert (CtxU (CtxU Γ A) (TyFun A C')) 2 A)
     as insertion. { simpl. destruct Γ; auto. }
-    rewrite insertion. apply c_insert_typesafe. assumption.
-    inv H. inv H0. inv H5. assumption.
+    rewrite insertion. apply c_insert_typesafe. auto.
+    inv H. inv H0. inv H5. auto.
 + destruct C as (A, Σ, E) eqn:e. apply shape_dobind in orig.
   destruct orig as [A' [c1ty]].
   apply TypeC. inv c1ty. 3 : eapply TypeDoBind. all: eauto. inv H. auto.
 + destruct C as (A, Σ, E) eqn:e. apply shape_dobind in orig.
   destruct orig as [A' [c1ty]]. eapply c_subs_out_typesafe. eauto.
-  apply shape_ret in c1ty. assumption.
+  apply shape_ret in c1ty. auto.
 + destruct C as (A, Σ, E) eqn:e. apply shape_dobind in orig.
   destruct orig as [A' [c1ty]]. eapply shape_op in c1ty.
   destruct c1ty as [Aop [Bop [gets [vty]]]]. apply TypeC.
-  - inv H. inv H1. assumption.
-  - inv H. assumption.
-  - eapply TypeOp; eauto. eapply TypeC. inv H0. assumption. inv H. assumption.
+  - inv H. inv H1. auto.
+  - inv H. auto.
+  - eapply TypeOp; eauto. eapply TypeC. inv H0. auto. inv H. auto.
     eapply TypeDoBind. exact H0.
-    assert (CtxU (CtxU Γ Bop) A' = ctx_insert (CtxU Γ A') Bop 1).
+    assert (CtxU (CtxU Γ Bop) A' = ctx_insert (CtxU Γ A') 1 Bop).
     { simpl. destruct Γ; auto. }
-    rewrite H1. apply c_insert_typesafe. assumption. inv H0. inv H2. assumption.
+    rewrite H1. apply c_insert_typesafe. auto. inv H0. inv H2. auto.
 + eapply shape_handle in orig. destruct orig as [C' [hty]]. 
-  apply TypeC. inv hty. assumption. inv hty. inv H1. assumption.
+  apply TypeC. inv hty. auto. inv hty. inv H1. auto.
   eapply TypeHandle; eauto.
 + eapply shape_handle in orig. rename C into D. destruct orig as [C[hty]].
   destruct C as (A, Σ, E). eapply shape_handler in hty as hty'. 
   destruct hty' as [Σ'[D'[retty[hcty[r[st]]]]]]. eapply shape_ret in H.
-  eapply c_subs_out_typesafe. 2:exact H. apply TypeC. 
-  - inv H. apply WfCtxU; assumption.
-  - inv hty. inv H2. assumption.
+  eapply c_subs_out_typesafe; eauto. apply TypeC. 
+  - inv H. apply WfCtxU; auto.
+  - inv hty. inv H2. auto.
   - eapply TypeCSubtype; eauto.
 + eapply shape_handle in orig. rename C into D. 
   destruct orig as [C[hty]]. destruct C as (A, Σ, E).
   eapply shape_handler in hty as hty'.
   destruct hty' as [Σ'[D'[retty[hcty[r[st]]]]]].
   eapply shape_op in H0 as opt. destruct opt as [Aop[Bop[gets]]].
-  assert (wf_ctx Γ) by (inv hty; assumption). 
-  apply TypeC; auto. inv hty. inv H5. assumption.
+  assert (wf_ctx Γ) by (inv hty; auto). 
+  apply TypeC; auto. inv hty. inv H5. auto.
   eapply TypeCSubtype; eauto. inv H2.
-  assert (wf_vtype Aop) by (inv H4; assumption).
-  assert (wf_vtype Bop) by (inv H5; inv H6; assumption).
-  assert (wf_ctype D') by (inv hcty; assumption).
-  unfold c_subs2_out. eapply c_subs_out_typesafe.
+  assert (wf_vtype Aop) by (inv H4; auto).
+  assert (wf_vtype Bop) by (inv H5; inv H6; auto).
+  assert (wf_ctype D') by (inv hcty; auto).
+  eapply c_subs_out_typesafe.
   instantiate (1:= TyFun Bop D').
-  unfold c_subs2_out. eapply c_subs_out_typesafe.
+  eapply c_subs_out_typesafe.
   instantiate (1:= Aop).
   - eapply sig_subtype_get_Some in gets; eauto.
     destruct gets as [A'[B'[gets']]]. inv H8.
@@ -128,24 +126,24 @@ induction step; intros C orig.
     * apply SubtypeCtxU. apply SubtypeCtxU.
       apply ctx_subtype_refl; auto. apply SubtypeTyFun; auto.
       apply csubtype_refl. all: auto.
-  - assert (CtxU Γ (TyFun Bop D') = ctx_insert Γ (TyFun Bop D') 0).
+  - assert (CtxU Γ (TyFun Bop D') = ctx_insert Γ 0 (TyFun Bop D')).
     { destruct Γ; simpl; reflexivity. }
     rewrite H8. eapply v_insert_typesafe. auto. apply WfTyFun; auto.
   - apply TypeV. auto. apply WfTyFun; auto.
     eapply TypeFun. apply TypeC. apply WfCtxU. all: auto.
     eapply TypeHandle. 2: exact H5.
-    assert (CtxU Γ Bop = ctx_insert Γ Bop 0) by (destruct Γ; simpl; auto).
+    assert (CtxU Γ Bop = ctx_insert Γ 0 Bop) by (destruct Γ; simpl; auto).
     rewrite H8. eapply v_insert_typesafe. 2: auto.
     apply TypeV. auto. apply WfTyHandler. inv H0. auto. auto.
     eapply TypeVSubtype. instantiate (1:=(TyHandler (CTy A Σ' E) D'));
     inv H5; inv H10; inv H0.
     * apply TypeV. auto. apply WfTyHandler. apply WfCTy; auto.
       all: try (inv hcty; assumption). eapply wf_eqs_sig_subtype; eauto.
-      inv hcty. assumption. apply TypeHandler; auto.
+      inv hcty. auto. apply TypeHandler; auto.
     * apply SubtypeTyHandler. apply SubtypeCTy. 2: auto.
       apply vsubtype_refl. inv H5. inv H10. auto.
       eapply eqs_subtype_refl. inv H5. inv H10. eauto.
-      apply csubtype_refl. assumption.
+      apply csubtype_refl. auto.
 Qed.
 
 (* ==================== Progress ==================== *)
